theories/Dot/lr/lr_lemmasDefs.v
@@ -6,57 +6,7 @@ Implicit Types (v: vl) (e: tm) (d: dm) (ds: dms) (Γ : ctx).
 Section Sec.
   Context `{HdlangG: dlangG Σ}.
 
-  Local Hint Resolve dms_lookup_head dms_lookup_mono : core.
   Local Arguments lift_dinterp_dms: simpl never.
-
-  Lemma lift_dinterp_dms_vl_commute T ds ρ l:
-    label_of_ty T = Some l →
-    lift_dinterp_dms LD⟦T⟧ ρ (selfSubst ds) -∗
-    lift_dinterp_vl l D*⟦T⟧ vnil ρ (vobj ds).
-  Proof.
-    rewrite /lift_dinterp_dms /=. iIntros (?).
-    iDestruct 1 as (?l d ?) "[% H]"; simplify_eq/=.
-    iExists d; iFrame. by iExists ds.
-  Qed.
-
-  Lemma lift_dsinterp_dms_vl_commute T ds ρ:
-    Ds⟦T⟧ ρ (selfSubst ds) -∗
-    ⟦T⟧ ρ (vobj ds).
-  Proof.
-    iIntros "H".
-    iInduction T as [] "IHT";
-      try iDestruct "H" as (???) "[_[]]"; first done.
-    - iDestruct "H" as "[#H1 #H2]".
-      by iSplit; [> iApply "IHT"| iApply "IHT1"].
-    - by rewrite (lift_dinterp_dms_vl_commute (TVMem _ _)).
-    - by rewrite (lift_dinterp_dms_vl_commute (TTMem _ _ _)).
-  Qed.
-
-  Lemma def2defs_head {T l ρ d ds}:
-    D[ l ]⟦T⟧ ρ d -∗
-    lift_dinterp_dms LD⟦T⟧ ρ ((l, d) :: ds).
-  Proof. iIntros; iExists l, d. auto. Qed.
-
-  Lemma lift_dinterp_dms_mono T l ρ d ds:
-    dms_hasnt ds l →
-    lift_dinterp_dms T ρ ds -∗
-    lift_dinterp_dms T ρ ((l, d) :: ds).
-  Proof.
-    intros ?. iDestruct 1 as (l' d' ?) "#H".
-    iExists l', d'. iSplit; auto.
-  Qed.
-
-  Lemma defs_interp_mono T l ρ d ds:
-    dms_hasnt ds l →
-    defs_interp T ρ ds -∗
-    defs_interp T ρ ((l, d) :: ds).
-  Proof.
-    iIntros (Hlds) "HT".
-    iInduction T as [] "IHT" => //=;
-      try by [iDestruct "HT" as (????) "?" | iApply lift_dinterp_dms_mono].
-    iDestruct "HT" as "[HT1 HT2]"; iSplit; by [>iApply "IHT"|iApply "IHT1"].
-  Qed.
-
   Local Arguments lift_dinterp_vl: simpl never.
   (* Local Arguments ldlty_car: simpl never. *)
   (* Local Arguments def_interp_tmem: simpl never.
@@ -125,10 +75,9 @@ Section Sec.
     iIntros (Hlds) "#HT1 [% #HT2]"; iSplit.
     by iIntros "!%"; cbn; constructor => //; by rewrite -dms_hasnt_notin_eq.
     iIntros "!>" (ρ [Hpid Hpids]%path_includes_split) "#Hg"; cbn.
-    iSpecialize ("HT1" $! _  Hpid with "Hg"). iPoseProof "HT1" as (Hl) "_".
+    iSpecialize ("HT1" $! _  Hpid with "Hg").
     iDestruct ("HT2" $! _  Hpids with "Hg") as "{HT2} HT2".
-    repeat iSplit.
-    - destruct T1; simplify_eq; iApply (def2defs_head with "HT1").
-    - iApply (defs_interp_mono with "HT2"); by [apply dms_hasnt_subst | eapply nclosed_sub_app].
+    iSplit; first by iApply def2defs_head.
+    iApply (defs_interp_mono with "HT2"); by [apply dms_hasnt_subst | eapply nclosed_sub_app].
   Qed.
 End Sec.
